HeapLang/Metatheory.thy
@@ -63,18 +63,128 @@ qed auto
 lemma is_closed_weaken_nil: "is_closed_expr {} e \<Longrightarrow> is_closed_expr X e"
   using is_closed_weaken by fastforce
 
-lemma is_closed_subst: "\<lbrakk>is_closed_val v; is_closed_expr (insert x X) e\<rbrakk> \<Longrightarrow> is_closed_expr X (subst x v e)"
-  "is_closed_val v \<Longrightarrow> is_closed_expr {} (Val v)"  
-proof (induction e and v arbitrary: X)
+lemma is_closed_subst: "\<lbrakk>is_closed_val v; is_closed_expr (insert x X) e\<rbrakk> \<Longrightarrow> is_closed_expr X (subst x v e)"  
+proof (induction e arbitrary: X)
   case (Rec x1 x2 e)
-  then show ?case 
-    by (smt (z3) cons_binder.simps(2) cons_binder_comm insertCI insert_absorb is_closed_expr.simps(3) subst.simps(3))
+  then show ?case
+    by (smt (verit, best) cons_binder.simps(2) cons_binder_comm insert_absorb2 is_closed_expr.simps(3) subst.simps(3))
 qed auto
 
 lemma is_closed_subst': "\<lbrakk>is_closed_val v; is_closed_expr (x#\<^sub>bX) e\<rbrakk> \<Longrightarrow> is_closed_expr X (subst' x v e)"
 using is_closed_subst subst'_def by (cases x) auto
 
+(* Substitution *)
 lemma subst_is_closed: "\<lbrakk>is_closed_expr X e; x \<notin> X\<rbrakk> \<Longrightarrow> subst x es e = e"
-sorry
+proof (induction e arbitrary: X)
+  case (Rec x1 x2 e)
+  then show ?case by (cases x1; cases x2) auto
+qed auto
+
+lemma subst_is_closed_nil: "is_closed_expr {} e \<Longrightarrow> subst x v e = e"
+using subst_is_closed by simp
+
+lemma subst_subst: "subst x v (subst x v' e) = subst x v' e"
+by (induction e) auto
+
+lemma subst_subst': "subst' x v (subst' x v' e) = subst' x v' e"
+by (cases x) (auto simp: subst'_def subst_subst)
+
+lemma subst_subst_ne: "x \<noteq> y \<Longrightarrow> subst x v (subst y v' e) = subst y v' (subst x v e)"
+by (induction e) auto
+
+lemma subst_subst_ne': "x \<noteq> y \<Longrightarrow> subst' x v (subst' y v' e) = subst' y v' (subst' x v e)"
+by (cases x; cases y) (auto simp: subst'_def subst_subst_ne)
+
+lemma subst_rec': "x = f \<or> x = y \<or> x = None \<Longrightarrow> subst' x v (Rec f y e) = Rec f y e"
+by (cases x) (auto simp: subst'_def)
+
+lemma subst_rec_ne': "\<lbrakk>x \<noteq> f \<or> f = None; x \<noteq> y \<or> y = None\<rbrakk> \<Longrightarrow>
+  subst' x v (Rec f y e) = Rec f y (subst' x v e)"
+  by (cases x) (auto simp: subst'_def)
+
+lemma bin_op_eval_closed: "\<lbrakk>is_closed_val v1; is_closed_val v2; bin_op_eval op v1 v2 = Some v'\<rbrakk> \<Longrightarrow>
+  is_closed_val v'" unfolding bin_op_eval_def by (cases op; auto split: val.splits base_lit.splits) 
+  (metis is_closed_val.simps(1) option.inject option.simps(3))
+
+
+definition map_forall :: "('a \<Rightarrow> 'b \<Rightarrow> bool) \<Rightarrow> ('a,'b) map \<Rightarrow> bool" where
+  "map_forall P m = (\<forall>k v. (m k = Some v) \<longrightarrow> P k v)"  
+
+definition option_map_or :: "('a \<Rightarrow> 'b) \<Rightarrow> 'b \<Rightarrow> 'a option \<Rightarrow> 'b" where
+  "option_map_or f b a = (case a of Some a \<Rightarrow> f a | None \<Rightarrow> b)"
+
+lemma heap_closed_alloc: "\<lbrakk>0 < n; is_closed_val w; 
+  map_forall (\<lambda>_ v. option_map_or is_closed_val True v) (heap \<sigma>);
+  (\<forall> i::int. (0 \<le> i) \<longrightarrow> (i < n) \<longrightarrow> heap \<sigma> (l +\<^sub>\<iota> i) = None)\<rbrakk> \<Longrightarrow>
+  map_forall (\<lambda>_ v. option_map_or is_closed_val True v) (heap \<sigma> ++ heap_array l (replicate (nat n) w))"
+  apply (auto simp: map_forall_def option_map_or_def loc_add_def split: option.splits)
+proof -
+  have "(heap_array l (replicate (nat n) w) k = Some (Some v)) \<Longrightarrow> w=v" for k v
+    using heap_array_lookup[of l "(replicate (nat n) w)" k v]
+    by (metis heap_array_elements in_set_replicate)
+  then show "\<And>k x2.
+    \<forall>k v. heap \<sigma> k = Some v \<longrightarrow> (\<forall>x2. v = Some x2 \<longrightarrow> is_closed_val x2) \<Longrightarrow>
+    \<forall>i\<ge>0. i < n \<longrightarrow> heap \<sigma> (Loc (loc_car l + i)) = None \<Longrightarrow> 0 < n \<Longrightarrow> is_closed_val w \<Longrightarrow> heap_array l (replicate (nat n) w) k = Some (Some x2) \<Longrightarrow> is_closed_val x2"
+    by blast
+qed
+
+
+lemma head_step_is_closed: "\<lbrakk> e1 \<sigma>1 obs \<Rightarrow>\<^sub>h e2 \<sigma>2 es; is_closed_expr {} e1; 
+  map_forall (\<lambda>_ v. option_map_or is_closed_val True v) (heap \<sigma>1)\<rbrakk> \<Longrightarrow>
+  is_closed_expr {} e2 \<and> list_all (is_closed_expr {}) es \<and>
+  map_forall (\<lambda>_ v. option_map_or is_closed_val True v) (heap \<sigma>2)"
+proof (induction rule: head_step.induct)
+  case (BetaS e' x v2 f e1 \<sigma>)
+  then show ?case using is_closed_subst' by force
+next
+  case (UnOpS op v v' \<sigma>)
+  then show ?case by (induction op v rule: un_op_eval.induct) auto
+next
+  case (BinOpS op v1 v2 v' \<sigma>)
+  then show ?case using bin_op_eval_closed is_closed_expr.simps(1,13) list_all_simps(2) by blast
+next
+  case (AllocNS n \<sigma> l v)
+  then show ?case
+    apply (auto simp: state_init_heap_def state_upd_heap_def split: option.splits)
+    apply (rule heap_closed_alloc[of n v \<sigma> l, OF AllocNS(1)])
+    by (auto simp: loc_add_def)
+next
+  case (NewProphS p \<sigma>)
+  then show ?case by (simp add: state_upd_used_proph_id_def)
+qed (auto simp: option_map_or_def map_forall_def subst'_def state_upd_heap_def split: option.splits)
+
+definition binder_delete :: "binder_t \<Rightarrow> (string,'a) map \<Rightarrow> (string,'a) map" where
+  "binder_delete b m = (case b of Some b \<Rightarrow> m(b:=None) | None \<Rightarrow> m)"
+
+fun subst_map :: "(string,val) map \<Rightarrow> expr \<Rightarrow> expr" where
+  "subst_map _ (Val v) = Val v"
+| "subst_map vs (Var y) = (case vs y of Some v \<Rightarrow> Val v | _ \<Rightarrow> Var y)"
+| "subst_map vs (Rec f y e) = Rec f y (subst_map (binder_delete y (binder_delete f vs)) e)"
+| "subst_map vs (App e1 e2) = App (subst_map vs e1) (subst_map vs e2)"
+| "subst_map vs (UnOp op e) = UnOp op (subst_map vs e)"
+| "subst_map vs (BinOp op e1 e2) = BinOp op (subst_map vs e1) (subst_map vs e2)"
+| "subst_map vs (If e0 e1 e2) = If (subst_map vs e0) (subst_map vs e1) (subst_map vs e2)"
+| "subst_map vs (Pair e1 e2) = Pair (subst_map vs e1) (subst_map vs e2)"
+| "subst_map vs (Fst e) = Fst (subst_map vs e)"
+| "subst_map vs (Snd e) = Snd (subst_map vs e)"
+| "subst_map vs (InjL e) = InjL (subst_map vs e)"
+| "subst_map vs (InjR e) = InjR (subst_map vs e)"
+| "subst_map vs (Case e0 e1 e2) = Case (subst_map vs e0) (subst_map vs e1) (subst_map vs e2)"
+| "subst_map vs (Fork e) = Fork (subst_map vs e)"
+| "subst_map vs (AllocN e1 e2) = AllocN (subst_map vs e1) (subst_map vs e2)"
+| "subst_map vs (Free e) = Free (subst_map vs e)"
+| "subst_map vs (Load e) = Load (subst_map vs e)"
+| "subst_map vs (Store e1 e2) = Store (subst_map vs e1) (subst_map vs e2)"
+| "subst_map vs (Xchg e1 e2) = Xchg (subst_map vs e1) (subst_map vs e2)"
+| "subst_map vs (CmpXchg e0 e1 e2) = CmpXchg (subst_map vs e0) (subst_map vs e1) (subst_map vs e2)"
+| "subst_map vs (FAA e1 e2) = FAA (subst_map vs e1) (subst_map vs e2)"
+| "subst_map vs NewProph = NewProph"
+| "subst_map vs (Resolve e0 e1 e2) = Resolve (subst_map vs e0) (subst_map vs e1) (subst_map vs e2)"
+
+lemma subst_map_empty: "subst_map Map.empty e = e"
+by (induction e) (auto simp: binder_delete_def split: option.splits)
+
+lemma subst_map_insert: "subst_map (vs(x\<mapsto>v)) e = subst x v (subst_map (vs(x:=None)) e)"
+by (induction e arbitrary: vs) (auto simp: binder_delete_def fun_upd_twist split: option.splits)
 
 end
